Replace definitions using HOL library's existing ones; update their lemmas; add closed term assumptions to some lemmas and proved them; TODO: need to add closed term assumption to correctness proofs for time and space models to fix them. (time model for sub machine is fixed; time model for heap machine, space model for sub and heap machines are not yet ffixed)

examples/lambda/wcbv-reasonable/AbstractHeapMachineScript.sml
@@ -22,6 +22,12 @@ Datatype:
   clos = closC Pro HA
 End
 
+(*
+  Inductive clos :=
+    closC (P:Pro) (a:HA).
+  Notation "P ! a" := (closC P a) (at level 40).
+*)
+
 Datatype:
   heapEntry = heapEntryC clos HA
 End
@@ -40,6 +46,18 @@ Definition extended:
   extended H H' =
     (∀alpha m. (get H alpha = SOME m) ⇒ (get H' alpha = SOME m))
 End
+
+(*
+  Inductive heapEntry := heapEntryC (g:clos) (alpha:HA).
+
+Heaps
+  Let Heap := list heapEntry.
+  Implicit Type H : Heap.
+  Definition put H e := (H++[e],|H|).
+  Definition get H alpha:= nth_error H alpha.
+  Definition extended H H' :=
+    forall alpha m, get H alpha = Some m -> get H' alpha = Some m.
+*)
 
 Theorem get_current:
   ∀H m H' alpha.
@@ -110,6 +128,22 @@ Inductive step:
     step (closC [] a::T, V, H) (T, V, H))
 End
 
+(*
+  Inductive step : state -> state -> Prop :=
+    step_pushVal P P' Q a T V H:
+      jumpTarget 0 [] P = Some (Q,P')
+      ->step ((lamT::P)!a::T,V,H) (P'!a::T,Q!a::V,H)
+  | step_beta a b g P Q H H' c T V:
+      put H (heapEntryC g b) = (H',c)
+      -> step ((appT::P)!a::T,g::Q!b::V,H) (Q!c ::P!a::T,V,H')
+  | step_load P a x g T V H:
+      lookup H a x = Some g
+      -> step ((varT x::P)!a::T,V,H) (P!a::T,g::V,H)
+  | step_nil a T V H: step ([]!a::T,V,H) (T,V,H).
+
+  Hint Constructors step.
+*)
+
 (* ------------------
         Unfolding
    ------------------ *)
@@ -160,44 +194,59 @@ Inductive reprC:
     unfolds H a 0 s s' ⇒
     reprC H (closC P a) s')
 End
+(*
+  Inductive reprC : Heap -> clos -> term -> Prop :=
+    reprCC H P s a s' :
+      reprP P s ->
+      unfolds H a 0 s s' ->
+      reprC H (P!a) s'.
+*)
 
+(* Add assumptions ``closed t'`` here
+    due to the difference between
+      how substitutions are defined
+        in HOL library and in Forster etc.'s Coq proof *)
 Theorem unfolds_subst':
   ∀H s s' t' a a' k g.
+    closed t' ⇒
     get H a' = SOME (heapEntryC g a) ⇒
     reprC H g t' ⇒
     unfolds H a (SUC k) s s' ⇒
     unfolds H a' k s (subst s' k t')
 Proof
   Induct_on `unfolds` >> rw[]
-    >- (rw[Once unfolds_cases] >> Cases_on `n < k` >> rw[]
-       >- rw[Once subst]
-        >> fs[NOT_LESS] >> rw[Once lookup] >>
-        `n ≤ k` by fs[LESS_EQ_IFF_LESS_SUC] >>
-        `n = k` by rw[] >> rw[] >>
-        fs[get] >> Cases_on `g` >> rw[] >>
-        fs[Once reprC_cases] >>
-       qexists_tac `s`  >> rw[] >>
-       rw[Once subst])
-    >- (rename [`lookup H a (n − SUC k) = SOME (closC P b)`,
+  >- (rw[Once unfolds_cases] >>
+      rw[Once lookup] >>
+      fs[get] >> Cases_on `g` >> rw[] >>
+      fs[Once reprC_cases] >>
+      qexists_tac `s`  >> rw[])
+  >- (rename [`lookup H a (n − SUC k) = SOME (closC P b)`,
                 `get H a' = SOME (heapEntryC g a)`] >>
-        `lookup H a' (n − k) = SOME (closC P b)`
-            by (Cases_on `n` >> rw[] >> fs[] >>
-                `lookup H a' (SUC (n' − k)) = SOME (closC P b)`
-                    suffices_by (rw[] >> fs[SUB_LEFT_SUC] >>
-                                 Cases_on `n' ≤ k` >> gs[] >>
-                                 `k = n'` by gs[integerTheory.INT_LE_ANTISYM] >>
-                                 rw[]) >>
-                rw[Once lookup]) >>
+      `lookup H a' (n − k) = SOME (closC P b)`
+        by (Cases_on `n` >> rw[] >> fs[] >>
+            `lookup H a' (SUC (n' − k)) = SOME (closC P b)`
+                suffices_by (rw[] >> fs[SUB_LEFT_SUC] >>
+                             Cases_on `n' ≤ k` >> gs[] >>
+                             `k = n'` by gs[integerTheory.INT_LE_ANTISYM] >>
+                              rw[]) >>
+            rw[Once lookup]) >>
         `bound k s'`
             by (drule unfolds_bound >> rw[] >>
                 `0 ≤ k` by simp[] >> metis_tac[bound_ge]) >>
         rw[bound_closed_k] >> rw[Once unfolds_cases] >> metis_tac[])
-    >- (rw[Once unfolds_cases] >> rw[Once subst])
-    >> rw[Once unfolds_cases] >> rw[Once subst]
+    >- ((* closed t' added for this subgoal *)
+        drule lift_closed >> rw[] >>
+        rw[Once unfolds_cases] >> metis_tac[ADD1])
+    >> rw[Once unfolds_cases] >> rw[]
 QED
 
+(* Add assumptions ``closed t'`` here
+    due to the difference between
+      how substitutions are defined
+        in HOL library and in Forster etc.'s Coq proof *)
 Theorem unfolds_subst:
   ∀H s s' t' a a' g.
+    closed t' ⇒
     get H a' = SOME (heapEntryC g a) ⇒
     reprC H g t' ⇒
     unfolds H a 1 s s' ⇒
@@ -225,6 +274,15 @@ A PreOrder is both Reflexive and Transitive.
     PreOrder_Reflexive :> Reflexive R | 2 ;
     PreOrder_Transitive :> Transitive R | 2 }.
  --------*)
+
+(*
+  Instance extended_PO :
+    PreOrder extended.
+  Proof.
+    unfold extended;split;repeat intro. all:eauto.
+  Qed.
+  Typeclasses Opaque extended.
+*)
 
 Theorem lookup_extend:
   ∀H H' a x g.
@@ -273,14 +331,16 @@ QED
 (* ------------------
           Time
    ------------------ *)
-
+(* TODO: fix time cost model *)
+(*
 Theorem correctTime':
   ∀s t k s0 P a T V H.
+  (*  closed ? ⇒*)
     timeBS k s t ⇒
     unfolds H a 0 s0 s ⇒
     ∃g l H'.
       reprC H' g t ∧
-      pow step l ((closC (compile s0++P) a)::T,V,H)
+      NRC step l ((closC (compile s0++P) a)::T,V,H)
         ((closC P a)::T,g::V,H') ∧
       l = 4*k+1 ∧
       extended H H'
@@ -339,39 +399,39 @@ Proof
   >- (`4 * k + 1 + ((4 * k' + 1) + ((4 * k'' + 1) + 1 + 1)) =
        4 * (k + (k' + (k'' + 1))) + 1`
         by rw[] >>
-      `pow step (4 * k + 1 + ((4 * k' + 1) + ((4 * k'' + 1) + 1 + 1)))
+      `NRC step (4 * k + 1 + ((4 * k' + 1) + ((4 * k'' + 1) + 1 + 1)))
           (closC (compile s'' ⧺ compile t1 ⧺ [appT] ⧺ P) a::T',V,H)
           (closC P a::T',g'::V,Heap3)`
         suffices_by rw[] >>
       pop_assum (K all_tac) >>
-      irule (iffRL pow_add) >> rw[Once rcomp] >>
+      irule (iffRL NRC_add) >> rw[Once rcomp] >>
       qexists_tac `(closC (compile t1 ⧺ appT::P) a::T',closC (compile s2) a2::V,Heap1)` >>
       rw[]
       >- (`compile s'' ⧺ compile t1 ⧺ appT::P = compile s'' ⧺ compile t1 ⧺ [appT] ⧺ P`
           suffices_by metis_tac[] >>
         rw[rich_listTheory.CONS_APPEND])
-      >> `pow step ((4 * k' + 1) + ((4 * k'' + 1) + 1 + 1))
+      >> `NRC step ((4 * k' + 1) + ((4 * k'' + 1) + 1 + 1))
           (closC (compile t1 ⧺ appT::P) a::T',closC (compile s2) a2::V,Heap1)
           (closC P a::T',g'::V,Heap3)`
           suffices_by rw[] >>
-      irule (iffRL pow_add) >> rw[Once rcomp] >>
+      irule (iffRL NRC_add) >> rw[Once rcomp] >>
       qexists_tac `(closC (appT::P) a::T',g::closC (compile s2) a2::V,Heap2)` >>
       rw[] >>
-      `pow step (1 + ((4 * k'' + 1) + 1))
+      `NRC step (1 + ((4 * k'' + 1) + 1))
           (closC (appT::P) a::T',g::closC (compile s2) a2::V,Heap2)
           (closC P a::T',g'::V,Heap3)`
         suffices_by rw[] >>
-      irule (iffRL pow_add) >> rw[Once rcomp] >>
+      irule (iffRL NRC_add) >> rw[Once rcomp] >>
       `step (closC (appT::P) a::T',g::closC (compile s2) a2::V,Heap2)
           (closC (compile s2) a2'::closC P a::T',V,Heap2')`
         by metis_tac[step_cases] >>
       qexists_tac `closC (compile s2) a2'::closC P a::T',V,Heap2'` >>
       rw[rcomp_1] >>
-      `pow step ((4 * k'' + 1) + 1)
+      `NRC step ((4 * k'' + 1) + 1)
         (closC (compile s2) a2'::closC P a::T',V,Heap2')
         (closC P a::T',g'::V,Heap3)`
         suffices_by rw[] >>
-      irule (iffRL pow_add) >> rw[Once rcomp] >>
+      irule (iffRL NRC_add) >> rw[Once rcomp] >>
       qexists_tac `(closC [] a2'::closC P a::T',g'::V,Heap3)` >>
       rw[] >>
       metis_tac[step_cases, rcomp_1])
@@ -392,7 +452,7 @@ Theorem correctTime:
   closed s ⇒
   ∃g H.
     reprC H g t
-    ∧ pow step (4*k+2) (init s)
+    ∧ NRC step (4*k+2) (init s)
                ([],[g],H)
 Proof
   rw[] >>
@@ -401,7 +461,7 @@ Proof
     unfolds H a 0 s0 s ⇒
     ∃g l H'.
       reprC H' g t ∧
-      pow step l ((closC (compile s0++P) a)::T,V,H)
+      NRC step l ((closC (compile s0++P) a)::T,V,H)
         ((closC P a)::T,g::V,H') ∧
       l = 4*k+1 ∧
       extended H H'`
@@ -413,13 +473,13 @@ Proof
   first_x_assum drule >> rw[] >>
   qexistsl_tac [`g`, `H'`] >> rw[] >>
   rw[init_def] >>
-  `pow step (4 * k + 1 + 1) ([closC (compile s) 0],[],[]) ([],[g],H')`
+  `NRC step (4 * k + 1 + 1) ([closC (compile s) 0],[],[]) ([],[g],H')`
     suffices_by rw[] >>
-  irule (iffRL pow_add) >> rw[Once rcomp] >>
+  irule (iffRL NRC_add) >> rw[Once rcomp] >>
   qexists_tac `([closC [] 0],[g],H')` >> rw[] >>
   metis_tac[step_cases, rcomp_1]
 QED
-
+*)
 (*
 
 Notation "a ! alpha" := (closC a alpha) (at level 40).
@@ -455,12 +515,12 @@ Section Analysis.
   Variable H: list heapEntry.
   Variable i : nat.
 
-  Hypothesis R: pow step i (init s) (T,V,H).
+  Hypothesis R: NRC step i (init s) (T,V,H).
 *)
 
 (*
 i s T V H
-pow step i (init s) (T,V,H) ∧
+NRC step i (init s) (T,V,H) ∧
 *)
 
 Theorem jumpTarget_eq':
@@ -510,7 +570,7 @@ then we have
 
 Theorem size_clos:
   ∀P a i s T V H.
-    pow step i (init s) (T,V,H) ⇒
+    NRC step i (init s) (T,V,H) ⇒
     (MEM (closC P a) (T++V) ⇒ sizeP P ≤ 2*size s ∧ a ≤ LENGTH H)
     ∧
     (∀beta.
@@ -521,27 +581,27 @@ Proof
   Induct_on `i` >> rw[]
   (* base cases *)
   (* 7 *)
-  >- (fs[pow, it_def, rcomp, Once step_cases, eq_cases, init_def] >>
+  >- (fs[NRC, it_def, rcomp, Once step_cases, eq_cases, init_def] >>
       gs[] >> rw[] >> metis_tac[sizeP_size])
-  >- (fs[pow, it_def, rcomp, Once step_cases, eq_cases, init_def] >>
+  >- (fs[NRC, it_def, rcomp, Once step_cases, eq_cases, init_def] >>
       gs[])
-  >- (fs[pow, it_def, rcomp, Once step_cases, eq_cases, init_def] >>
+  >- (fs[NRC, it_def, rcomp, Once step_cases, eq_cases, init_def] >>
       gs[])
-  >- (fs[pow, it_def, rcomp, Once step_cases, eq_cases, init_def] >>
+  >- (fs[NRC, it_def, rcomp, Once step_cases, eq_cases, init_def] >>
       gs[])
-  >- (fs[pow, it_def, rcomp, Once step_cases, eq_cases, init_def] >>
+  >- (fs[NRC, it_def, rcomp, Once step_cases, eq_cases, init_def] >>
       gs[])
-  >- (fs[pow, it_def, rcomp, Once step_cases, eq_cases, init_def] >>
+  >- (fs[NRC, it_def, rcomp, Once step_cases, eq_cases, init_def] >>
       gs[])
-  >- (fs[pow, it_def, rcomp, Once step_cases, eq_cases, init_def] >>
+  >- (fs[NRC, it_def, rcomp, Once step_cases, eq_cases, init_def] >>
       gs[])
   (* Inductive cases *)
   (* 7 *)
   (* MEM (closC P a) T' *)
     (* ==> SUM (MAP sizeT P) + 1 ≤ 2 * size s *)
-  >- (fs[ADD1] >> drule (iffLR pow_add) >> rw[] >>
+  >- (fs[ADD1] >> drule (iffLR NRC_add) >> rw[] >>
       pop_assum mp_tac >> rw[Once rcomp] >>
-      rename [`pow step 1 y (T',V,H)`] >>
+      rename [`NRC step 1 y (T',V,H)`] >>
       `step y (T', V, H)` by metis_tac[rcomp_1] >>
       PairCases_on `y` >> gs[] >>
       first_x_assum drule >> rw[] >>
@@ -568,9 +628,9 @@ Proof
           >> metis_tac[])
       >> fs[] >> metis_tac[])
     (* a ≤ LENGTH H *)
-  >- (fs[ADD1] >> drule (iffLR pow_add) >> rw[] >>
+  >- (fs[ADD1] >> drule (iffLR NRC_add) >> rw[] >>
       pop_assum mp_tac >> rw[Once rcomp] >>
-      rename [`pow step 1 y (T',V,H)`] >>
+      rename [`NRC step 1 y (T',V,H)`] >>
       `step y (T', V, H)` by metis_tac[rcomp_1] >>
       PairCases_on `y` >> gs[] >>
       first_x_assum drule >> rw[] >>
@@ -585,9 +645,9 @@ Proof
       >> fs[] >> rw[] >> metis_tac[])
   (* MEM (closC P a) V *)
     (* SUM (MAP sizeT P) + 1 ≤ 2 * size s *)
-  >- (fs[ADD1] >> drule (iffLR pow_add) >> rw[] >>
+  >- (fs[ADD1] >> drule (iffLR NRC_add) >> rw[] >>
       pop_assum mp_tac >> rw[Once rcomp] >>
-      rename [`pow step 1 y (T',V,H)`] >>
+      rename [`NRC step 1 y (T',V,H)`] >>
       `step y (T', V, H)` by metis_tac[rcomp_1] >>
       PairCases_on `y` >> gs[] >>
       first_x_assum drule >> rw[] >>
@@ -607,9 +667,9 @@ Proof
           fs[] >> rw[] >> metis_tac[])
       >> fs[] >> metis_tac[])
     (* a ≤ LENGTH H *)
-  >- (fs[ADD1] >> drule (iffLR pow_add) >> rw[] >>
+  >- (fs[ADD1] >> drule (iffLR NRC_add) >> rw[] >>
       pop_assum mp_tac >> rw[Once rcomp] >>
-      rename [`pow step 1 y (T',V,H)`] >>
+      rename [`NRC step 1 y (T',V,H)`] >>
       `step y (T', V, H)` by metis_tac[rcomp_1] >>
       PairCases_on `y` >> gs[] >>
       first_x_assum drule >> rw[] >>
@@ -623,9 +683,9 @@ Proof
       >> fs[] >> metis_tac[])
   (* MEM (heapEntryC (closC P a) beta) H *)
     (* SUM (MAP sizeT P) + 1 ≤ 2 * size s *)
-  >- (fs[ADD1] >> drule (iffLR pow_add) >> rw[] >>
+  >- (fs[ADD1] >> drule (iffLR NRC_add) >> rw[] >>
       pop_assum mp_tac >> rw[Once rcomp] >>
-      rename [`pow step 1 y (T',V,H)`] >>
+      rename [`NRC step 1 y (T',V,H)`] >>
       `step y (T', V, H)` by metis_tac[rcomp_1] >>
       PairCases_on `y` >> gs[] >>
       first_x_assum drule >> rw[] >>
@@ -636,9 +696,9 @@ Proof
           fs[] >> rw[] >> metis_tac[])
       >> fs[] >> metis_tac[])
     (* a ≤ LENGTH H *)
-  >- (fs[ADD1] >> drule (iffLR pow_add) >> rw[] >>
+  >- (fs[ADD1] >> drule (iffLR NRC_add) >> rw[] >>
       pop_assum mp_tac >> rw[Once rcomp] >>
-      rename [`pow step 1 y (T',V,H)`] >>
+      rename [`NRC step 1 y (T',V,H)`] >>
       `step y (T', V, H)` by metis_tac[rcomp_1] >>
       PairCases_on `y` >> gs[] >>
       first_x_assum drule >> rw[] >>
@@ -651,9 +711,9 @@ Proof
           fs[] >> rw[] >> metis_tac[])
       >> fs[] >> metis_tac[])
     (* beta ≤ LENGTH H *)
-  >- (fs[ADD1] >> drule (iffLR pow_add) >> rw[] >>
+  >- (fs[ADD1] >> drule (iffLR NRC_add) >> rw[] >>
       pop_assum mp_tac >> rw[Once rcomp] >>
-      rename [`pow step 1 y (T',V,H)`] >>
+      rename [`NRC step 1 y (T',V,H)`] >>
       `step y (T', V, H)` by metis_tac[rcomp_1] >>
       PairCases_on `y` >> gs[] >>
       first_x_assum drule >> rw[] >>
@@ -669,15 +729,15 @@ QED
 
 Theorem length_H:
   ∀i s T V H.
-    pow step i (init s) (T,V,H) ⇒
+    NRC step i (init s) (T,V,H) ⇒
     LENGTH H ≤ i
 Proof
   Induct_on `i` >> rw[ADD1]
-  >- (fs[pow, it_def, rcomp, init_def] >>
+  >- (fs[NRC, it_def, rcomp, init_def] >>
       drule (iffLR eq_cases) >> rw[])
-  >> drule (iffLR pow_add) >> rw[] >>
+  >> drule (iffLR NRC_add) >> rw[] >>
   pop_assum mp_tac >> rw[Once rcomp] >>
-  rename [`pow step 1 y (T',V,H)`] >>
+  rename [`NRC step 1 y (T',V,H)`] >>
   `step y (T', V, H)` by metis_tac[rcomp_1] >>
   PairCases_on `y` >> gs[] >>
   first_x_assum drule >> rw[] >>
@@ -688,15 +748,15 @@ QED
 
 Theorem length_TV:
   ∀i s T V H.
-    pow step i (init s) (T,V,H) ⇒
+    NRC step i (init s) (T,V,H) ⇒
     LENGTH T + LENGTH V <= 1+i
 Proof
   Induct_on `i` >> rw[ADD1]
-  >- (fs[pow, it_def, rcomp, init_def] >>
+  >- (fs[NRC, it_def, rcomp, init_def] >>
       drule (iffLR eq_cases) >> rw[])
-  >> drule (iffLR pow_add) >> rw[] >>
+  >> drule (iffLR NRC_add) >> rw[] >>
   pop_assum mp_tac >> rw[Once rcomp] >>
-  rename [`pow step 1 y (T',V,H)`] >>
+  rename [`NRC step 1 y (T',V,H)`] >>
   `step y (T', V, H)` by metis_tac[rcomp_1] >>
   PairCases_on `y` >> gs[] >>
   first_x_assum drule >> rw[] >>
@@ -740,9 +800,18 @@ Proof
   rw[integerTheory.INT_LDISTRIB]
 QED
 
+  (*
+  Lemma list_bound X size m (A:list X):
+    (forall x, x el A -> size x <= m) -> sum (map size A) <= length A * m.
+  Proof.
+    induction A;cbn;intros H'. omega.
+    rewrite IHA. rewrite H'. omega. tauto. intuition.
+  Qed.
+  *)
+(* TODO *)
 Theorem correctSpace:
   ∀i s T V H.
-    pow step i (init s) (T,V,H) ⇒
+    NRC step i (init s) (T,V,H) ⇒
     sizeSt (T,V,H) ≤ (i + 1) * (3*i+4*size s)
 Proof
   rw[sizeSt_def, sizeH_def] >>
@@ -803,4 +872,149 @@ Proof
   >> rw[Abbr `b`, Abbr `d`]
 QED
 
+(*
+End Analysis.
+*)
+
+(* --------------------------------
+    Bonus: Unfolding on Programs
+   -------------------------------- *)
+(*
+Bonus: Unfolding on Programs
+We define a function f to unfold a closure, needed for the Turing machine M_unf.
+Section UnfoldPro.
+
+  Variable H : list heapEntry.
+
+  Fixpoint f (P:Pro) a k fuel {struct fuel}: option Pro :=
+    match fuel with
+      0 => None
+    | S fuel =>
+      match P,k with
+       (* retT,0 => Some retT *)
+      | retT::P,S k =>
+        match f P a k fuel with
+          Some P' => Some (retT::P')
+        | _ => None
+        end
+      | appT::P,_ =>
+        match f P a k fuel with
+          Some P' => Some (appT::P')
+        | _ => None
+        end
+      | lamT::P,_ =>
+        match f P a (S k) fuel with
+          Some P' => Some (lamT::P')
+        | _ => None
+        end
+      | varT n::P,_ =>
+        if Dec (n >= k) then
+          match lookup H a (n-k) with
+            Some (closC Q b) =>
+            match f Q b 1 fuel,f P a k fuel with
+              Some Q', Some P' =>
+              Some (lamT::Q'++retT::P')
+            | _,_ => None
+            end
+          | _ => None
+          end
+        else
+          match f P a k fuel with
+            Some P' =>
+            Some (varT n::P')
+          | _ => None
+          end
+      |[],_ => Some []
+      |_,_ => None
+      end
+    end.
+
+  Lemma f_mono P a k n n' :
+    n <= n' -> f P a k n <> None -> f P a k n' = f P a k n.
+  Proof.
+    induction n in P,a,k,n'|-*. now cbn.
+    destruct n'. now omega.
+    intros leq eq. cbn in eq|-*.
+    repeat (let eq := fresh "eq" in destruct _ eqn:eq).
+    all:try congruence.
+    all: repeat match goal with
+            _ : S ?n <= S ?n',
+                H : (f ?P ?a ?k ?n' = _) ,
+                    H' : (f ?P ?a ?k ?n = _)
+            |- _ => rewrite IHn in H;[ | omega | congruence]
+                    end.
+    all:congruence.
+  Qed.
+  Lemma f_correct' Q Q' a k s s' n:
+    unfolds H a k s s' ->
+    f Q a k n = Some Q' ->
+    exists n', f (compile s++Q) a k n' = Some (compile s' ++ Q').
+  Proof.
+    induction s' in Q',Q,a,k,s,n |- *;intros H' eq.
+    inv H'.
+    - exists (S n). cbn. decide _. omega.
+      now rewrite eq.
+    - cbn. exfalso. inv H2. inv H3.
+    - inv H'.
+      {exfalso. inv H2. inv H3. }
+      cbn [compile].
+      autorewrite with list.
+      edestruct IHs'2 with (Q:=appT::Q) (n:=S n) as [n2 eq2]. 1:eassumption.
+      cbn. now rewrite eq.
+      edestruct IHs'1 as [n1 eq1]. 1:eassumption.
+      2:{
+        eexists. erewrite eq1. reflexivity.
+      }
+      eassumption.
+    -inv H'.
+     +inv H2. inv H3.
+      edestruct IHs' with (n:=1)(Q:=@nil Tok) as [n1 eq1]. eassumption.
+      reflexivity.
+      autorewrite with list in eq1.
+      exists (S (max n n1)).
+      cbn. decide _. 2:omega. rewrite H1. erewrite f_mono.
+      rewrite eq1. erewrite f_mono. rewrite eq.
+      autorewrite with list. reflexivity.
+      1,3:now apply Nat.max_case_strong;omega.
+      1-2:congruence.
+     + cbn. edestruct IHs' as [n1 eq1].
+       3:{eexists (S _).
+       cbn.
+       autorewrite with list.
+       cbn. rewrite eq1. reflexivity. }
+       eassumption.
+       instantiate (1 := S n).
+       cbn. rewrite eq. now destruct Q.
+  Qed.
+  Lemma f_correct a s s' k:
+    unfolds H a k s s' ->
+    exists n', f (compile s) a k n' = Some (compile s').
+  Proof.
+    intros H'.
+    specialize (f_correct' (n:=1) (Q:=@nil Tok) (Q':=@nil Tok) H') as [n eq].
+    reflexivity.
+    autorewrite with list in eq.
+    eexists. rewrite eq. reflexivity.
+  Qed.
+  Lemma f_correct_final P a s:
+    reprC H (P!a) s ->
+    exists t, s = lam t /\ exists n, f P a 1 n = Some (compile t).
+  Proof.
+    intros H'. inv H'. inv H4. inv H6.
+    specialize (f_correct H2) as eq. eauto.
+  Qed.
+End UnfoldPro.
+
+Lemma unfolds_inj H k s a s1 s2 :
+  unfolds H k s a s1 -> unfolds H k s a s2 -> s1=s2.
+Proof.
+  induction 1 in s2|-*;intros H';inv H';try congruence;try omega.
+  -apply IHunfolds.
+   replace b with b0 in * by congruence.
+   inv H2. inv H7.
+   replace s1 with s in * by (apply compile_inj;congruence). tauto.
+  -f_equal. apply IHunfolds. auto.
+  -f_equal. all:auto.
+Qed.
+*)
 val _ = export_theory ()
